lib/CompileConfRelSimplified.v
@@ -12,17 +12,17 @@ Import HListNotations.
 Section CompileConfRelSimplified.
   Set Implicit Arguments.
   (* State identifiers. *)
-  Variable (S: Type).
-  Context `{S_eq_dec: EquivDec.EqDec S eq}.
-  Context `{S_finite: @Finite S _ S_eq_dec}.
+  Variable (St: Type).
+  Context `{St_eq_dec: EquivDec.EqDec St eq}.
+  Context `{St_finite: @Finite St _ St_eq_dec}.
 
   (* Header identifiers. *)
-  Variable (H: Type).
-  Context `{H_eq_dec: EquivDec.EqDec H eq}.
-  Context `{H_finite: @Finite H _ H_eq_dec}.
-  Variable (sz: H -> nat).
+  Variable (Hdr: Type).
+  Context `{Hdr_eq_dec: EquivDec.EqDec Hdr eq}.
+  Context `{Hdr_finite: @Finite Hdr _ Hdr_eq_dec}.
+  Variable (sz: Hdr -> nat).
 
-  Variable (a: P4A.t S sz).
+  Variable (a: P4A.t St sz).
 
   Fixpoint compile_bctx (b: bctx): ctx (sig sz) :=
     match b with
@@ -30,7 +30,7 @@ Section CompileConfRelSimplified.
     | BCSnoc b size => CSnoc _ (compile_bctx b) (Bits size)
     end.
 
-  Definition be_sort {c} b1 b2 (e: bit_expr H c) : sorts :=
+  Definition be_sort {c} b1 b2 (e: bit_expr Hdr c) : sorts :=
     Bits (be_size sz b1 b2 e).
 
   Equations compile_var {c: bctx} (x: bvar c) : var (sig sz) (compile_bctx c) (Bits (check_bvar x)) :=
@@ -100,7 +100,7 @@ Section CompileConfRelSimplified.
   Equations compile_bit_expr
             {c: bctx}
             (b1 b2: nat)
-            (e: bit_expr H c)
+            (e: bit_expr Hdr c)
     : tm (sig sz) (app_ctx (outer_ctx b1 b2) (compile_bctx c)) (be_sort b1 b2 e) :=
     { compile_bit_expr b1 b2 (BELit _ _ l) :=
         TFun (sig sz) (BitsLit _ (List.length l) (Ntuple.l2t l)) hnil;
@@ -128,7 +128,7 @@ Section CompileConfRelSimplified.
   Equations compile_store_rel
             {c: bctx}
             (b1 b2: nat)
-            (r: store_rel H c)
+            (r: store_rel Hdr c)
             : fm (sig sz) (app_ctx (outer_ctx b1 b2) (compile_bctx c)) :=
     { compile_store_rel b1 b2 BRTrue := FTrue;
       compile_store_rel b1 b2 BRFalse := FFalse;
@@ -153,7 +153,7 @@ Section CompileConfRelSimplified.
 
   Definition compile_simplified_conf_rel
     (b1 b2: nat)
-    (r: simplified_conf_rel H)
+    (r: simplified_conf_rel Hdr)
     : fm (sig sz) (outer_ctx b1 b2)
   :=
     let sr: fm (sig sz) _ :=
@@ -163,7 +163,7 @@ Section CompileConfRelSimplified.
 
   Definition compile_simplified_crel
     (b1 b2: nat)
-    (R: simplified_crel H)
+    (R: simplified_crel Hdr)
     : fm (sig sz) (outer_ctx b1 b2) :=
     List.fold_right (fun r f =>
       FAnd _ (compile_simplified_conf_rel b1 b2 r) f
@@ -210,7 +210,7 @@ Section CompileConfRelSimplified.
   Qed.
 
   Lemma compile_bit_expr_correct:
-    forall c (e: bit_expr H c) bval b1 b2 buf1 buf2 store1 store2,
+    forall c (e: bit_expr Hdr c) bval b1 b2 buf1 buf2 store1 store2,
       interp_bit_expr e bval buf1 buf2 store1 store2 =
       let valu := outer_valu buf1 buf2 store1 store2 in
       interp_tm (m := fm_model a) (app_valu _ valu (compile_bval bval))
@@ -235,7 +235,7 @@ Section CompileConfRelSimplified.
   Qed.
 
   Lemma compile_store_rel_correct:
-    forall c (r: store_rel H c) bval b1 b2 buf1 buf2 store1 store2,
+    forall c (r: store_rel Hdr c) bval b1 b2 buf1 buf2 store1 store2,
       interp_store_rel r bval buf1 buf2 store1 store2 <->
       let valu := outer_valu buf1 buf2 store1 store2 in
       interp_fm (m := fm_model a) (app_valu _ valu (compile_bval bval))
@@ -304,8 +304,8 @@ Section CompileConfRelSimplified.
     intuition.
     unfold outer_ctx in valu.
     repeat dependent destruction valu.
-    simpl in m0, m1, m2, m3.
-    now apply H4.
+    simpl in *.
+    eauto.
   Qed.
 
   Lemma compile_simplified_entailment_correct':
@@ -326,8 +326,8 @@ Section CompileConfRelSimplified.
     intuition.
     unfold outer_ctx in valu.
     repeat dependent destruction valu.
-    simpl in m0, m1, m2, m3.
-    now apply H4.
+    simpl in *.
+    eauto.
   Qed.
 
   Opaque interp_fm.
