lib/Sum.v
@@ -13,37 +13,37 @@ Section Sum.
   Set Implicit Arguments.
 
   (* State identifiers. *)
-  Variable (S1: Type).
-  Context `{S1_eq_dec: EquivDec.EqDec S1 eq}.
-  Context `{S1_finite: @Finite S1 _ S1_eq_dec}.
+  Variable (St1: Type).
+  Context `{St1_eq_dec: EquivDec.EqDec St1 eq}.
+  Context `{St1_finite: @Finite St1 _ St1_eq_dec}.
 
-  Variable (S2: Type).
-  Context `{S2_eq_dec: EquivDec.EqDec S2 eq}.
-  Context `{S2_finite: @Finite S2 _ S2_eq_dec}.
+  Variable (St2: Type).
+  Context `{St2_eq_dec: EquivDec.EqDec St2 eq}.
+  Context `{St2_finite: @Finite St2 _ St2_eq_dec}.
 
   (* Header identifiers. *)
-  Variable (H1: Type).
-  Variable (sz1 : H1 -> nat).
-  Context `{H1_eq_dec: EquivDec.EqDec H1 eq}.
-  Context `{H1_finite: @Finite H1 _ H1_eq_dec}.
+  Variable (Hdr1: Type).
+  Variable (sz1 : Hdr1 -> nat).
+  Context `{Hdr1_eq_dec: EquivDec.EqDec Hdr1 eq}.
+  Context `{Hdr1_finite: @Finite Hdr1 _ Hdr1_eq_dec}.
 
-  Variable (H2: Type).
-  Variable (sz2 : H2 -> nat).
-  Context `{H2_eq_dec: EquivDec.EqDec H2 eq}.
-  Context `{H2_finite: @Finite H2 _ H2_eq_dec}.
+  Variable (Hdr2: Type).
+  Variable (sz2 : Hdr2 -> nat).
+  Context `{Hdr2_eq_dec: EquivDec.EqDec Hdr2 eq}.
+  Context `{Hdr2_finite: @Finite Hdr2 _ Hdr2_eq_dec}.
 
-  Variable (a1: Syntax.t S1 sz1).
-  Variable (a2: Syntax.t S2 sz2).
+  Variable (a1: Syntax.t St1 sz1).
+  Variable (a2: Syntax.t St2 sz2).
 
-  Notation S := (S1 + S2)%type.
+  Notation St := (St1 + St2)%type.
 
-  Global Instance S_eq_dec: EquivDec.EqDec S eq :=
+  Global Instance St_eq_dec: EquivDec.EqDec St eq :=
     ltac:(typeclasses eauto).
 
-  Global Instance S_finite: @Finite S _ S_eq_dec :=
+  Global Instance St_finite: @Finite St _ St_eq_dec :=
     ltac:(typeclasses eauto).
 
-  Definition H : Type := H1 + H2.
+  Definition H : Type := Hdr1 + Hdr2.
 
   Definition make_transparent {X: Type} (eq_dec: forall (x0 x1: X), {x0 = x1} + {x0 <> x1}) {l r} (opaque_eq: l = r) : l = r :=
     match eq_dec l r with
@@ -57,7 +57,7 @@ Section Sum.
     | inr h => sz2 h
     end.
 
-  Program Definition sum : Syntax.t S sz :=
+  Program Definition sum : Syntax.t St sz :=
     {| Syntax.t_states s :=
          match s with
          | inl s1 => Syntax.state_fmapSH sz inl inl _ (a1.(Syntax.t_states) s1)
